\documentclass{article}
\usepackage[english]{babel}
\usepackage{geometry}
\geometry{letterpaper}

\begin{document}

3. Example. (a) Recall that an O.U. process is a stationary Gaussian process
with mean zero and covariance given by $r (s, t) = \sigma^2 \exp [- \beta |s -
t|]$ for $0 \leq s, t \leq a$ where $\beta > 0, \sigma^2 > 0$ are constants.
If $\beta_i, \sigma^2_i, i = 1, 2$ relate to a pair of O.U. processes, so that
$r_i = u_i v_i$ with $u_i (t) = \sigma^2_i \exp (\beta_i t), v_i (t) = \exp (-
\beta_i t)$ then the conditions given in the theorem show that the measures
$P_0^{r_i}, i = 1, 2$ are equivalent iff $\sigma^2_1 \beta_1 = \sigma^2_2
\beta_2 = K$ (say). The likelihood ratio is then obtained from (2) as follows
where $D_1, D_2$ and the integrand, denoted $f$, are found to be:
\begin{equation}
  D^2_1 = \frac{\beta_2}{\beta_1}, \quad D_2 = \frac{2}{K}  (\beta_1 -
  \beta_2)
\end{equation}
and
\begin{equation}
  f = - \frac{(\beta_2 - \beta_1)}{K} \exp [- (\beta_1 + \beta_2) t]
\end{equation}
Substituting these in (2) and using integration by parts one gets
\[ \frac{dP_0^{r 2}}{dP_0^{r 1}} (X) = \sqrt{\frac{\beta_2}{\beta_1}} \exp \{-
   \frac{1}{2 K} [(\beta_2 - \beta_1) (X^2 (0) + X^2 (a)) + (\beta^2_2 -
   \beta^2_1) \int_0^a X^2 (t) \hspace{0.17em} dt]\} \]
This example is also discussed by Striebel [1]. [There is a small numerical
discrepancy here.] See also Duttweiler and Kailath [1],[2], Kailath and
Weinert [1], and Kailath, Geesy and Weinert [1], for related work.

(b) An even simpler example is noted for the equivalence of the BM and the
Brownian bridge both have means zero and covariances $r_1  (s, t) = \min (s,
t)$ and $r_2  (s, t) = u (s \wedge t) v (s \vee t)$ for $0 \leq s, t \leq a <
1$ where $u (s) = s, v (s) = 1 - s$. In this case $D^2_1 = \frac{1}{1 - a},
D_2 = 0, f (t) = - 1$

\end{document}
