$$
\frac{1}{2} \int_{-\infty}^{\infty} C(x)r_n(x) \, dx = \frac{1}{2} \int_{-\infty}^{\infty} p_n(-a)S(a) \, da
$$

$p_n(a)$ are even functions, so $p_n(-a) = p_n(a)$:

$$
\frac{1}{2} \int_{-\infty}^{\infty} p_n(-a)S(a) \, da = \frac{1}{2} \int_{-\infty}^{\infty} p_n(a)S(a) \, da
$$

Orthogonality condition:

$$
\int_{-\infty}^{\infty} p_n(a)p_m(a)S(a) \, da = \delta_{nm}
$$

For $n \neq 0$:

$$
\int_{-\infty}^{\infty} p_n(a)S(a) \, da = 0
$$

Therefore:

$$
\frac{1}{2} \int_{-\infty}^{\infty} C(x)r_n(x) \, dx = 0 \quad \text{for } n \neq 0
$$

