\documentclass[11pt]{article}
\usepackage{amsmath,amsthm,amssymb,amsfonts}
\usepackage{geometry}
\geometry{margin=1in}

\newtheorem{theorem}{Theorem}
\newtheorem{lemma}{Lemma}
\newtheorem{proposition}{Proposition}
\newtheorem{definition}{Definition}
\newtheorem{corollary}{Corollary}

\title{Injectively Time-Changed Stationary Processes}
\author{}
\date{}

\begin{document}
\maketitle

\begin{definition}
An \emph{injectively time-changed stationary process} is a stochastic process $\{X(t)\}_{t \in \mathbb{R}}$ with spectral representation
\begin{equation}
X(t) = \int_{-\infty}^{\infty} e^{i\lambda\theta(t)} \, dZ(\lambda)
\end{equation}
where $\theta: \mathbb{R} \to \mathbb{R}$ is strictly increasing, $\theta \in C^1(\mathbb{R})$, and $\{Z(\lambda)\}_{\lambda \in \mathbb{R}}$ is an orthogonal increment process with $E[|dZ(\lambda)|^2] = F(d\lambda)$.
\end{definition}

\begin{proposition}
\begin{equation}
X(t) = \int_{-\infty}^{\infty} A(t,\lambda) e^{i\lambda t} \, dZ(\lambda)
\end{equation}
where
\begin{equation}
A(t,\lambda) = e^{i\lambda(\theta(t)-t)}
\end{equation}
\end{proposition}

\begin{proof}
\begin{align}
X(t) &= \int_{-\infty}^{\infty} e^{i\lambda\theta(t)} \, dZ(\lambda)\\
&= \int_{-\infty}^{\infty} e^{i\lambda(\theta(t)-t)} e^{i\lambda t} \, dZ(\lambda)
\end{align}
\end{proof}

\begin{theorem}
\begin{enumerate}
\item $E[|X(t)|^2] = \int_{-\infty}^{\infty} F(d\lambda) < \infty$
\item $\text{Cov}(X(s),X(t)) = \int_{-\infty}^{\infty} e^{i\lambda(\theta(s)-\theta(t))} F(d\lambda)$
\end{enumerate}
\end{theorem}

\begin{proof}
\begin{align}
E[|X(t)|^2] &= \int_{-\infty}^{\infty} |e^{i\lambda\theta(t)}|^2 F(d\lambda) = \int_{-\infty}^{\infty} F(d\lambda)\\
\text{Cov}(X(s),X(t)) &= \int_{-\infty}^{\infty} e^{i\lambda\theta(s)} \overline{e^{i\lambda\theta(t)}} F(d\lambda)\\
&= \int_{-\infty}^{\infty} e^{i\lambda(\theta(s)-\theta(t))} F(d\lambda)
\end{align}
\end{proof}

\begin{theorem}
$X(t)$ is stationary if and only if $\theta(t) = t + c$ for some $c \in \mathbb{R}$.
\end{theorem}

\begin{proof}
($\Leftarrow$) If $\theta(t) = t + c$:
\begin{equation}
\text{Cov}(X(s),X(t)) = \int_{-\infty}^{\infty} e^{i\lambda c} e^{-i\lambda c} F(d\lambda) = \int_{-\infty}^{\infty} F(d\lambda)
\end{equation}

($\Rightarrow$) Stationarity requires $\theta(s) - \theta(t) = g(s-t)$. Differentiating: $\theta'(s) = g'(s-t)$. Both sides constant implies $\theta'(t) = k$, so $\theta(t) = kt + c$. Covariance depending only on $s-t$ requires $k = 1$.
\end{proof}

\begin{definition}
$\Delta(t) := \theta(t) - t$
\end{definition}

\begin{proposition}
\begin{enumerate}
\item $\Delta'(t) = \theta'(t) - 1$
\item $A(t,\lambda) = e^{i\lambda\Delta(t)}$
\item Instantaneous frequency: $\frac{d}{dt}[\lambda\theta(t)] = \lambda\theta'(t)$
\end{enumerate}
\end{proposition}

\begin{theorem}
If $\theta$ has inverse $\psi$ and $F(d\lambda) = f(\lambda)d\lambda$:
\begin{equation}
f(\lambda) = \lim_{T \to \infty} \frac{1}{2T} \int_{-T}^T X(\psi(u)) e^{-i\lambda u} \frac{du}{\psi'(u)}
\end{equation}
\end{theorem}

\begin{proof}
Substitution $u = \theta(t)$:
\begin{equation}
X(\psi(u)) = \int_{-\infty}^{\infty} e^{i\mu u} dZ(\mu)
\end{equation}
Standard inversion formula applies with measure transformation factor $\frac{1}{\psi'(u)}$.
\end{proof}

\begin{theorem}
If $|\theta(s) - \theta(t)| \to \infty$ as $|t-s| \to \infty$ and $F$ is absolutely continuous:
\begin{equation}
\lim_{|t-s| \to \infty} \text{Cov}(X(s),X(t)) = 0
\end{equation}
\end{theorem}

\begin{proof}
Riemann-Lebesgue lemma applied to
\begin{equation}
\text{Cov}(X(s),X(t)) = \int_{-\infty}^{\infty} e^{i\lambda(\theta(s)-\theta(t))} F(d\lambda)
\end{equation}
\end{proof}

\begin{corollary}[Band-Limited Case]
When $F$ has support in $[-B,B]$:
\begin{equation}
X(t) = \int_{-B}^B e^{i\lambda\theta(t)} \, dZ(\lambda)
\end{equation}
\end{corollary}

\end{document}
