\documentclass{article}
\usepackage{amsmath,amsthm,amssymb}

\newtheorem{theorem}{Theorem}

\begin{document}

\begin{theorem}[Inverse Filter for Unitary Time Transformations]
\label{thm:inverse-filter}
Let $\theta: \mathbb{R} \to \mathbb{R}$ be absolutely continuous, strictly increasing, and bijective with $\theta'(t) > 0$ almost everywhere. Let $Y(u)$ be a stationary process with unit variance, and define
\[
Z(t) = \sqrt{\theta'(t)} \, Y(\theta(t))
\]
as the oscillatory process obtained by the unitary time transformation. Then:
\begin{enumerate}
\item \label{item:forward}
The forward filter kernel is
\[
h(t,u) = \sqrt{\theta'(t)} \, \delta(u - \theta(t)).
\]

\item \label{item:inverse}
The inverse filter kernel is
\[
g(t,s) = \frac{\delta(s - \theta^{-1}(t))}{\sqrt{\theta'(\theta^{-1}(t))}}.
\]

\item \label{item:composition}
The composition $(g \circ h)$ recovers the identity:
\[
Y(t) = \int_{\mathbb{R}} g(t,s) Z(s) \, ds = \frac{Z(\theta^{-1}(t))}{\sqrt{\theta'(\theta^{-1}(t))}}.
\]
\end{enumerate}
\end{theorem}

\begin{proof}
We establish parts \ref{item:forward}--\ref{item:composition} in sequence.

\textbf{Part \ref{item:forward}.}
From the definition of $Z(t)$,
\[
Z(t) = \sqrt{\theta'(t)} \, Y(\theta(t)) = \int_{\mathbb{R}} \sqrt{\theta'(t)} \, \delta(u - \theta(t)) \, Y(u) \, du,
\]
so $h(t,u) = \sqrt{\theta'(t)} \, \delta(u - \theta(t))$.

\textbf{Part \ref{item:inverse}.}
Define
\[
g(t,s) = \frac{\delta(s - \theta^{-1}(t))}{\sqrt{\theta'(\theta^{-1}(t))}}.
\]
To verify it is the inverse filter, compute:
\[
\int_{\mathbb{R}} g(t,s) Z(s) \, ds
  = \int_{\mathbb{R}} \frac{\delta(s - \theta^{-1}(t))}{\sqrt{\theta'(\theta^{-1}(t))}} \, \sqrt{\theta'(s)} \, Y(\theta(s)) \, ds.
\]
Let $v = \theta(s)$, so $s = \theta^{-1}(v)$ and $ds = \frac{dv}{\theta'(\theta^{-1}(v))}$. Then
\[
= \int_{\mathbb{R}} 
  \frac{\delta(\theta^{-1}(v) - \theta^{-1}(t))}{\sqrt{\theta'(\theta^{-1}(t))}} \,
  \sqrt{\theta'(\theta^{-1}(v))} \,
  Y(v) \,
  \frac{dv}{\theta'(\theta^{-1}(v))}.
\]
Simplify:
\[
= \int_{\mathbb{R}} 
  \frac{\delta(\theta^{-1}(v) - \theta^{-1}(t))}{\sqrt{\theta'(\theta^{-1}(t))}\sqrt{\theta'(\theta^{-1}(v))}} 
  \, Y(v) \, dv.
\]
Using the identity
\[
\delta(\theta^{-1}(v) - \theta^{-1}(t)) = \theta'(\theta^{-1}(t)) \, \delta(v - t),
\]
we obtain
\[
= \int_{\mathbb{R}}
\frac{\theta'(\theta^{-1}(t)) \, \delta(v - t)}{\sqrt{\theta'(\theta^{-1}(t))}\sqrt{\theta'(\theta^{-1}(v))}} \, Y(v) \, dv.
\]
Evaluating at $v = t$,
\[
= Y(t).
\]
Thus $g(t,s) = \frac{\delta(s - \theta^{-1}(t))}{\sqrt{\theta'(\theta^{-1}(t))}}$ is the correct inverse kernel.

\textbf{Part \ref{item:composition}.}
Substituting $Z$ explicitly yields
\[
Y(t)
  = \int_{\mathbb{R}} g(t,s) Z(s) \, ds
  = \int_{\mathbb{R}} \frac{\delta(s - \theta^{-1}(t))}{\sqrt{\theta'(\theta^{-1}(t))}} \, Z(s) \, ds
  = \frac{Z(\theta^{-1}(t))}{\sqrt{\theta'(\theta^{-1}(t))}}.
\]
Hence $(g \circ h)(t,u)$ acts as the identity transformation in $L^2(\mathbb{R})$.
\end{proof}

\end{document}
