\documentclass{article}
\usepackage{amsmath}
\usepackage{amssymb}
\usepackage{amsthm}
\usepackage{amsfonts}
\usepackage{hyperref}

\newtheorem{theorem}{Theorem}
\newtheorem{lemma}{Lemma}
\newtheorem{corollary}{Corollary}
\newtheorem{definition}{Definition}
\newtheorem{proof}{Proof}

\title{Oscillatory Processes: General Theory and Injective Time Change Subclass}
\author{}
\date{}

\begin{document}

\maketitle

\section{General Oscillatory Process Theory}

\begin{theorem}[Oscillatory Process Spectral Representation]\label{thm:spectral}
An oscillatory process $X(t)$ admits the representation
\[
X(t) = \int_{-\infty}^{\infty} \phi_t(\lambda) dZ(\lambda) = \int_{-\infty}^{\infty} A(t,\lambda) e^{i\lambda t} dZ(\lambda)
\]
where $\phi_t(\lambda) = A(t,\lambda) e^{i\lambda t}$ is the oscillatory function, $A(t,\lambda)$ is the time-varying gain function satisfying:
\begin{enumerate}
\item \label{cond:measurable} $A(t,\lambda)$ is measurable in both arguments,
\item \label{cond:L2} $\int_{-\infty}^{\infty} |A(t,\lambda)|^2 dF(\lambda) < \infty$ for all finite $t \in \mathbb{R}$,
\end{enumerate}
and $dZ(\lambda)$ is a complex orthogonal increment process with $\mathbb{E}[dZ(\lambda_1) d\overline{Z(\lambda_2)}] = \delta(\lambda_1 - \lambda_2) dF(\lambda_1)$.

The covariance kernel is
\[
K(t,s) = \mathbb{E}[X(t)\overline{X(s)}] = \int_{-\infty}^{\infty} A(t,\lambda) \overline{A(s,\lambda)} e^{i\lambda(t-s)} dF(\lambda)
\]
\end{theorem}

\begin{proof}
\begin{align}
K(t,s) &= \mathbb{E}[X(t)\overline{X(s)}] \\
&= \mathbb{E}\left[\int_{-\infty}^{\infty} A(t,\lambda_1) e^{i\lambda_1 t} dZ(\lambda_1) \int_{-\infty}^{\infty} \overline{A(s,\lambda_2) e^{i\lambda_2 s} dZ(\lambda_2)}\right] \\
&= \int_{-\infty}^{\infty} \int_{-\infty}^{\infty} A(t,\lambda_1) \overline{A(s,\lambda_2)} e^{i(\lambda_1 t - \lambda_2 s)} \mathbb{E}[dZ(\lambda_1) d\overline{Z(\lambda_2)}] \\
&= \int_{-\infty}^{\infty} A(t,\lambda) \overline{A(s,\lambda)} e^{i\lambda(t-s)} dF(\lambda)
\end{align}
\end{proof}

\begin{theorem}[Time-Varying Filter Representation]\label{thm:filter}
An oscillatory process $X(t)$ can be represented as
\[
X(t) = \int_{-\infty}^{\infty} h(t,u) Y(t-u) du
\]
where $Y(t)$ is stationary with spectral representation $Y(t) = \int_{-\infty}^{\infty} e^{i\lambda t} dZ(\lambda)$, and the time-varying impulse response satisfies
\[
h(t,u) = \frac{1}{2\pi} \int_{-\infty}^{\infty} A(t,\lambda) e^{-i\lambda u} d\lambda
\]
\[
A(t,\lambda) = \int_{-\infty}^{\infty} h(t,u) e^{i\lambda u} du
\]
provided the integrals exist.
\end{theorem}

\begin{theorem}[Kernel Recovery: Mean Square Convergence]\label{thm:kernel}
For an oscillatory process $X(t)$ with gain function $A(t,\lambda)$ and underlying stationary ergodic process $Y(t) = \int_{-\infty}^{\infty} e^{i\lambda t} dZ(\lambda)$, the covariance kernel can be recovered from a single sample path as
\[
K(t,s) = \lim_{T \to \infty} \frac{1}{T} \int_0^T X(u+t) \overline{X(u+s)} du
\]
in mean square, provided:
\begin{enumerate}
\item \label{cond:uniformL2} $\sup_{t \in \mathbb{R}} \int_{-\infty}^{\infty} |A(t,\lambda)|^2 dF(\lambda) < \infty$
\item \label{cond:uniformBound} $\sup_{t \in \mathbb{R}} \sup_{\lambda \in \mathbb{R}} |A(t,\lambda)| < \infty$
\item \label{cond:unifCont} $A(t,\lambda)$ is uniformly continuous in $t$ for each $\lambda$
\item \label{cond:ergodic} $Y(t)$ is stationary and ergodic
\end{enumerate}
\end{theorem}

\begin{proof}
Define the time-averaged covariance estimator:
\[
\hat{K}_T(t,s) = \frac{1}{T} \int_0^T X(u+t) \overline{X(u+s)} du
\]
We establish mean square convergence $\mathbb{E}[|\hat{K}_T(t,s) - K(t,s)|^2] \to 0$ as $T \to \infty$.

Using the spectral representation:
\begin{align}
\hat{K}_T(t,s) &= \frac{1}{T} \int_0^T \int_{-\infty}^{\infty} \int_{-\infty}^{\infty} A(u+t,\lambda_1) \overline{A(u+s,\lambda_2)} e^{i(\lambda_1(u+t) - \lambda_2(u+s))} dZ(\lambda_1) d\overline{Z(\lambda_2)} du \\
&= \int_{-\infty}^{\infty} \int_{-\infty}^{\infty} \left(\frac{1}{T} \int_0^T A(u+t,\lambda_1) \overline{A(u+s,\lambda_2)} e^{i(\lambda_1(u+t) - \lambda_2(u+s))} du\right) dZ(\lambda_1) d\overline{Z(\lambda_2)}
\end{align}

For the integral kernel, define:
\[
I_T(\lambda_1,\lambda_2) = \frac{1}{T} \int_0^T A(u+t,\lambda_1) \overline{A(u+s,\lambda_2)} e^{i(\lambda_1(u+t) - \lambda_2(u+s))} du
\]

When $\lambda_1 = \lambda_2 = \lambda$:
\[
I_T(\lambda,\lambda) = e^{i\lambda(t-s)} \frac{1}{T} \int_0^T A(u+t,\lambda) \overline{A(u+s,\lambda)} du
\]

By the uniform boundedness (\ref{cond:uniformBound}) and uniform continuity (\ref{cond:unifCont}), the bounded convergence theorem applies to the sequence
\[
\frac{1}{T} \int_0^T A(u+t,\lambda) \overline{A(u+s,\lambda)} du
\]
yielding
\[
\lim_{T \to \infty} \frac{1}{T} \int_0^T A(u+t,\lambda) \overline{A(u+s,\lambda)} du = A(t,\lambda) \overline{A(s,\lambda)}
\]

When $\lambda_1 \neq \lambda_2$, the oscillatory factor $e^{i(\lambda_1 - \lambda_2)u}$ causes $I_T(\lambda_1,\lambda_2) \to 0$ as $T \to \infty$ under (\ref{cond:uniformBound}).

Using the orthogonality condition $\mathbb{E}[dZ(\lambda_1) d\overline{Z(\lambda_2)}] = \delta(\lambda_1 - \lambda_2) dF(\lambda_1)$:
\[
\lim_{T \to \infty} \mathbb{E}[\hat{K}_T(t,s)] = \int_{-\infty}^{\infty} A(t,\lambda) \overline{A(s,\lambda)} e^{i\lambda(t-s)} dF(\lambda) = K(t,s)
\]

Condition (\ref{cond:uniformL2}) ensures the variance $\mathbb{E}[|\hat{K}_T(t,s) - K(t,s)|^2] \to 0$, completing the proof.
\end{proof}

\section{Injective Time Change Subclass}

\begin{definition}[Injective Time Change Process]\label{def:injective}
An injective time change oscillatory process is defined as $X(t) = Y(\theta(t))$ where $Y(t)$ is stationary and $\theta(t)$ is strictly monotonic. The corresponding gain function is $A(t,\lambda) = \exp(i\lambda(\theta(t) - t))$.
\end{definition}

\begin{lemma}[Measure of Fixed Points]\label{lem:fixedpts}
For $\theta(t)$ strictly monotonic and continuous, the set $S = \{t : \theta(t) = t\}$ is at most countable. If $\theta(t)$ is strictly increasing (decreasing) and $\theta(t) \neq t$ for all $t$, then $S = \emptyset$.
\end{lemma}

\begin{proof}
If $\theta$ is strictly increasing and continuous, then $f(t) = \theta(t) - t$ is continuous. The zeros of a continuous function on $\mathbb{R}$ form a closed set with no accumulation points unless the function is identically zero. Since $\theta(t) \neq t$ for all $t$ by assumption, $S = \emptyset$.
\end{proof}

\begin{theorem}[Spectral Concentration for Injective Time Change]\label{thm:specconc}
For the injective time change process with $A(t,\lambda) = \exp(i\lambda(\theta(t) - t))$ where $\theta(t)$ is strictly monotonic, the gain function satisfies $|A(t,\lambda)| = 1$ for all $t,\lambda$, ensuring uniform spectral concentration.
\end{theorem}

\begin{proof}
Direct calculation: $|A(t,\lambda)| = |\exp(i\lambda(\theta(t) - t))| = 1$ for all $t,\lambda \in \mathbb{R}$.
\end{proof}

\begin{theorem}[Kernel Recovery for Injective Time Change]\label{thm:injkernel}
For the injective time change process $X(t) = Y(\theta(t))$ where $Y(t)$ is stationary and ergodic, and $\theta(t)$ is strictly monotonic with $\sup_{t \in \mathbb{R}} |\theta'(t)| < \infty$, the kernel can be recovered as:
\[
K(t,s) = \lim_{T \to \infty} \frac{1}{T} \int_0^T X(u+t) \overline{X(u+s)} du
\]
in mean square.
\end{theorem}

\begin{proof}
The conditions of Theorem~\ref{thm:kernel} are satisfied:
\begin{enumerate}
\item By Theorem~\ref{thm:specconc}, $\sup_{t \in \mathbb{R}} \int_{-\infty}^{\infty} |A(t,\lambda)|^2 dF(\lambda) = \int_{-\infty}^{\infty} dF(\lambda) < \infty$
\item By Theorem~\ref{thm:specconc}, $\sup_{t \in \mathbb{R}} \sup_{\lambda \in \mathbb{R}} |A(t,\lambda)| = 1 < \infty$
\item $A(t,\lambda) = \exp(i\lambda(\theta(t) - t))$ is uniformly continuous in $t$ when $\sup_{t} |\theta'(t)| < \infty$
\item $Y(t)$ is stationary and ergodic by assumption
\end{enumerate}
Therefore, kernel recovery holds by Theorem~\ref{thm:kernel}.
\end{proof}

\begin{corollary}[Explicit Kernel Formula]\label{cor:explicit}
For the injective time change process, the recovered kernel is:
\[
K(t,s) = \int_{-\infty}^{\infty} e^{i\lambda(\theta(t) - \theta(s))} dF(\lambda) = R_Y(\theta(t) - \theta(s))
\]
where $R_Y$ is the covariance function of the underlying stationary process $Y$.
\end{corollary}

\begin{proof}
Direct substitution of $A(t,\lambda) = \exp(i\lambda(\theta(t) - t))$ into the kernel formula from Theorem~\ref{thm:spectral}:
\[
K(t,s) = \int_{-\infty}^{\infty} \exp(i\lambda(\theta(t) - t)) \exp(-i\lambda(\theta(s) - s)) e^{i\lambda(t-s)} dF(\lambda) = \int_{-\infty}^{\infty} e^{i\lambda(\theta(t) - \theta(s))} dF(\lambda)
\]
Since $X(t) = Y(\theta(t))$, $K(t,s) = \mathbb{E}[Y(\theta(t))\overline{Y(\theta(s))}] = R_Y(\theta(t) - \theta(s))$.
\end{proof}

\end{document}
