\documentclass{article}
\usepackage[english]{babel}
\usepackage{amsmath,amssymb,latexsym}

%%%%%%%%%% Start TeXmacs macros
\newenvironment{proof}{\noindent\textbf{Proof\ }}{\hspace*{\fill}$\Box$\medskip}
\newtheorem{lemma}{Lemma}
\newtheorem{theorem}{Theorem}
%%%%%%%%%% End TeXmacs macros

\begin{document}

\begin{theorem}
  [Recovery of the Random Spectral Measure] Let $S_t$ be a second-order
  stationary process with spectral representation
  \begin{equation}
    S_t = \int_{- \infty}^{\infty} e^{i \omega t} \, dZ (\omega)
  \end{equation}
  where $Z (\omega)$ is the spectral process with orthogonal increments $dZ
  (\omega)$ satisfying $E [|dZ (\omega)|^2] = d\mu (\omega)$. Let $\theta :
  \mathbb{R} \to \mathbb{R}$ be smooth, strictly increasing, with $\theta'(t) > 0$, and define the time-changed process
  \begin{equation}
    X_t = \sqrt{\theta'(t)}\, S_{\theta(t)}
  \end{equation}
  Then for any $a < b$, the spectral increment $Z(b) - Z(a)$ can be recovered from the observed sample path $X_t$ via
  \begin{equation}
    Z(b) - Z(a) = \lim_{T \to \infty} \frac{1}{\sqrt{2T}} \int_{\tau(-T)}^{\tau(T)} X_t \sqrt{\theta'(t)} \left[ \int_a^b e^{-i\omega\theta(t)} d\omega \right] dt
  \end{equation}
  where $\tau = \theta^{-1}$ and the limit is a regular limit.
\end{theorem}

\begin{proof}
  Substitute the spectral representation into $X_t$:
  \begin{equation}
    X_t = \sqrt{\theta'(t)} \int_{-\infty}^\infty e^{i\omega\theta(t)} dZ(\omega)
  \end{equation}
  Consider
  \begin{align}
    Y_T &= \frac{1}{\sqrt{2T}} \int_{\tau(-T)}^{\tau(T)} X_t \sqrt{\theta'(t)} \left[ \int_a^b e^{-i\omega\theta(t)} d\omega \right] dt \\
    &= \frac{1}{\sqrt{2T}} \int_{\tau(-T)}^{\tau(T)} \theta'(t) \int_{-\infty}^\infty e^{i\xi\theta(t)} dZ(\xi) \left[ \int_a^b e^{-i\omega\theta(t)} d\omega \right] dt\\
    &= \frac{1}{\sqrt{2T}} \int_{-\infty}^\infty dZ(\xi)\int_{\tau(-T)}^{\tau(T)} \theta'(t) e^{i\xi\theta(t)} \left[ \int_a^b e^{-i\omega\theta(t)} d\omega \right] dt
  \end{align}
  Make the substitution $u = \theta(t)$, $du = \theta'(t)\,dt$, and note as $T\to\infty$, the integration range in $u$ covers $(-T,T)$. Then:
  \begin{align}
    Y_T &= \frac{1}{\sqrt{2T}} \int_{-\infty}^\infty dZ(\xi) \int_{-T}^T e^{i\xi u} \left[ \int_a^b e^{-i\omega u} d\omega \right] du\\
    &= \frac{1}{\sqrt{2T}} \int_{-\infty}^\infty dZ(\xi) \int_{-T}^T \int_a^b e^{i(\xi-\omega)u} d\omega\, du\\
    &= \frac{1}{\sqrt{2T}} \int_{-\infty}^\infty dZ(\xi) \int_a^b \int_{-T}^T e^{i(\xi-\omega)u} du\, d\omega\\
    &= \frac{1}{\sqrt{2T}} \int_{-\infty}^\infty dZ(\xi) \int_a^b \frac{2\sin((\xi-\omega)T)}{(\xi-\omega)} d\omega
  \end{align}
  As $T \to \infty$, the function $\frac{\sin((\xi-\omega)T)}{\xi-\omega}$ converges to $\pi\delta(\xi-\omega) T$ in the distributional sense, and so
  \begin{align}
    \lim_{T \to \infty} Y_T = \int_a^b dZ(\omega) = Z(b) - Z(a)
  \end{align}
  which completes the proof.
\end{proof}

\begin{lemma}
  [Mathematical Necessity of the $\sqrt{2T}$ Factor] The normalization factor $1 / \sqrt{2T}$ in the recovery formula is determined by the requirement that
  \begin{equation}
    \lim_{T \to \infty} E \left[ \left| \frac{1}{\sqrt{2T}} \int_{-T}^T S_s e^{-i\omega s} ds \right|^2 \right] = d\mu(\omega)
  \end{equation}
\end{lemma}

\begin{proof}
  Let $Y_T(\omega) = \frac{1}{\sqrt{2T}} \int_{-T}^T S_s e^{-i\omega s} ds$. By the spectral representation, $S_s = \int e^{i\xi s} dZ(\xi)$:
  \begin{align}
    E\left[|Y_T(\omega)|^2\right] &= \frac{1}{2T} E\left|\int_{-\infty}^\infty dZ(\xi) \int_{-T}^T e^{i(\xi-\omega)s} ds\right|^2\\
    &= \frac{1}{2T} \int_{-\infty}^\infty \left|\int_{-T}^T e^{i(\xi-\omega)s} ds\right|^2 d\mu(\xi)
  \end{align}
  The inner integral is $\frac{2\sin((\xi-\omega)T)}{\xi-\omega}$, so
  \begin{equation}
    E\left[|Y_T(\omega)|^2\right] = \frac{2}{T} \int_{-\infty}^\infty \frac{\sin^2((\xi-\omega)T)}{(\xi-\omega)^2} d\mu(\xi)
  \end{equation}
  As $T\to\infty$, $\frac{\sin^2(uT)}{\pi T u^2} \to \delta(u)$ in the sense of distributions, so
  \begin{equation}
    \lim_{T\to\infty} E\left[|Y_T(\omega)|^2\right] = d\mu(\omega)
  \end{equation}
  Thus $1/\sqrt{2T}$ is the correct normalization.
\end{proof}

\end{document}