\documentclass{article}
\usepackage[english]{babel}
\usepackage{amsmath,latexsym}

%%%%%%%%%% Start TeXmacs macros
\newcommand{\tmaffiliation}[1]{\\ #1}
\newcommand{\tmtextbf}[1]{\text{{\bfseries{#1}}}}
\newenvironment{proof}{\noindent\textbf{Proof\ }}{\hspace*{\fill}$\Box$\medskip}
\newtheorem{theorem}{Theorem}
%%%%%%%%%% End TeXmacs macros

%


\begin{document}

\title{Oscillatory Process Inversion}

\author{
  Stephen Crowley
  \tmaffiliation{September 30, 2025}
}

\maketitle

\begin{theorem}
  [Inversion of Oscillatory Processes]\label{thm:inversion}Given
  \begin{equation}
    Z (s) = \int_{- \infty}^{\infty} \phi_s (\lambda)  \hspace{0.17em} d \Phi
    (\lambda)
  \end{equation}
  where $\phi_s (\lambda)$ is measurable, invertible ($\phi_s (\lambda) \neq
  0$ for all $s, \lambda$), and satisfies the \tmtextbf{quadratic
  integrability condition}:
  \begin{equation}
    \int_{- \infty}^{\infty} \int_{- \infty}^{\infty} | \phi_t (\lambda) |^2 
    \hspace{0.17em} dt \hspace{0.17em} d \lambda < \infty
  \end{equation}
  and $\Phi (\lambda)$ is a complex orthogonal random measure with
  \begin{equation}
    E (|d \Phi (\lambda) |^2) = d \mu (\lambda)
  \end{equation}
  Define the stationary process:
  \begin{equation}
    X (t) = \int_{- \infty}^{\infty} e^{i \lambda t}  \hspace{0.17em} d \Phi
    (\lambda)
  \end{equation}
  Define the inverse kernel:
  \begin{equation}
    \label{eq:inverse-kernel} b (t, s) = \frac{1}{2 \pi}  \int_{-
    \infty}^{\infty} \frac{e^{i \lambda t}}{\phi_s (\lambda)}  \hspace{0.17em}
    e^{- i \lambda s}  \hspace{0.17em} d \lambda
  \end{equation}
  \tmtextbf{Invertibility condition:} Require
  \begin{equation}
    \label{eq:invertibility} \int_{- \infty}^{\infty} \int_{- \infty}^{\infty}
    \left| \frac{1}{\phi_t (\lambda)} \right|^2  \hspace{0.17em} dt
    \hspace{0.17em} d \lambda < \infty
  \end{equation}
  Then:
  \begin{equation}
    \label{eq:inversion-formula} X (t) = \int_{- \infty}^{\infty} b (t, s) 
    \hspace{0.17em} Z (s)  \hspace{0.17em} ds
  \end{equation}
\end{theorem}

\begin{proof}
  \begin{itemize}
    \item \label{step:expand} Expand the convolution:
    \begin{equation}
      \begin{array}{ll}
        \int_{- \infty}^{\infty} b (t, s)  \hspace{0.17em} Z (s) 
        \hspace{0.17em} ds & = \int_{- \infty}^{\infty} \left[ \frac{1}{2 \pi}
        \int_{- \infty}^{\infty} \frac{e^{i \lambda t}}{\phi_s (\lambda)}
        e^{- i \lambda s} d \lambda \right]\\
        & \quad \times \left[ \int_{- \infty}^{\infty} \phi_s (\omega) d \Phi
        (\omega) \right] ds
      \end{array}
    \end{equation}
    \item \label{step:fubini} Exchange order of integration by Fubini's
    theorem (justified by the quadratic integrability conditions
    \eqref{eq:invertibility}):
    \begin{equation}
      \begin{array}{ll}
        & = \frac{1}{2 \pi}  \int_{- \infty}^{\infty} \int_{-
        \infty}^{\infty} \left[ \int_{- \infty}^{\infty} e^{i \lambda t} 
        \frac{\phi_s (\omega)}{\phi_s (\lambda)} e^{- i \lambda s} ds \right]
        d \lambda \hspace{0.17em} d \Phi (\omega)
      \end{array}
    \end{equation}
    \item \label{step:inner-integral} Evaluate the inner integral over $s$:
    \begin{equation}
      \int_{- \infty}^{\infty} \frac{\phi_s (\omega)}{\phi_s (\lambda)} e^{- i
      \lambda s} ds
    \end{equation}
    For $\phi_s (\lambda) = A_s (\lambda) e^{i \lambda s}$:
    \begin{equation}
      \frac{\phi_s (\omega)}{\phi_s (\lambda)} e^{- i \lambda s} = \frac{A_s
      (\omega)}{A_s (\lambda)} e^{i (\omega - \lambda) s}
    \end{equation}
    The integral becomes:
    \begin{equation}
      \label{eq:dirac-delta} \int_{- \infty}^{\infty} \frac{A_s (\omega)}{A_s
      (\lambda)} e^{i (\omega - \lambda) s}  \hspace{0.17em} ds = 2 \pi
      \hspace{0.17em} \delta (\omega - \lambda)
    \end{equation}
    where this holds as a distributional identity under the stated
    integrability and invertibility conditions.
    
    \item \label{step:substitute} Substitute \eqref{eq:dirac-delta} back:
    \begin{equation}
      \begin{array}{ll}
        \frac{1}{2 \pi}  \int_{- \infty}^{\infty} \int_{- \infty}^{\infty}
        e^{i \lambda t} \cdot 2 \pi \delta (\omega - \lambda)  \hspace{0.17em}
        d \lambda \hspace{0.17em} d \Phi (\omega) & = \int_{- \infty}^{\infty}
        e^{i \omega t}  \hspace{0.17em} d \Phi (\omega)\\
        & = X (t)
      \end{array}
    \end{equation}
  \end{itemize}
  
\end{proof}

\section*{Summary}

Under the conditions:
\begin{enumerate}
  \item $\int \int | \phi_t (\lambda) |^2  \hspace{0.17em} dt \hspace{0.17em}
  d \lambda < \infty$
  
  \item $\phi_s (\lambda) \neq 0$ everywhere
  
  \item $\int \int |1 / \phi_t (\lambda) |^2  \hspace{0.17em} dt
  \hspace{0.17em} d \lambda < \infty$
\end{enumerate}
The stationary process $X (t)$ is exactly inverted from the oscillatory
process $Z (t)$ by equation \eqref{eq:inversion-formula} with kernel
\eqref{eq:inverse-kernel}.

\end{document}
