\documentclass{article}
\usepackage{amsmath}

\title{The Logarithmic Derivative of Bessel Functions}
\author{}
\date{}

\begin{document}
\maketitle

The Bessel function $J_n(t)$ satisfies:
\[
t^2J_n''(t) + tJ_n'(t) + (t^2 - n^2)J_n(t) = 0
\]

Its logarithmic derivative is:
\[
w(t) = \frac{J_n'(t)}{J_n(t)}
\]

The logarithmic derivative satisfies a Riccati equation, as follows:

\begin{enumerate}
\item The definition directly implies:
    \[J_n'(t) = w(t)J_n(t)\]

\item The derivative of this equation is:
    \[J_n''(t) = w'(t)J_n(t) + w(t)^2J_n(t)\]

\item These expressions in the Bessel equation yield:
    \[t^2(w'(t)J_n(t) + w(t)^2J_n(t)) + t(w(t)J_n(t)) + (t^2 - n^2)J_n(t) = 0\]

\item Division by $J_n(t)$ produces:
    \[t^2w'(t) + t^2w(t)^2 + tw(t) + (t^2 - n^2) = 0\]

\item The equation rearranges to:
    \[w'(t) = -w(t)^2 - \frac{w(t)}{t} - (1 - \frac{n^2}{t^2})\]
\end{enumerate}

The logarithmic derivative of $J_n(t)$ satisfies this Riccati equation.

\end{document}
