\documentclass{article}
\usepackage[english]{babel}
\usepackage{geometry}
\geometry{letterpaper}

\begin{document}

\

\section*{Riemann-Siegel Formula}

The exact Riemann-Siegel formula for the Riemann zeta function on the critical
line, with the remainder term as an infinite sum, is:
\begin{equation}
  \zeta (\frac{1}{2} + it) = \sum_{n = 1}^N \frac{1}{n^{1 / 2 + it}} + \chi
  (t)  \sum_{n = 1}^N \frac{1}{n^{1 / 2 - it}} + R (t)
\end{equation}
Where:
\begin{itemize}
  \item $N = \lfloor \sqrt{\frac{t}{2 \pi}} \rfloor$
  
  \item 
\end{itemize}
The remainder term $R (t)$ is given by the exact infinite sum:
\begin{equation}
  R (t) = \frac{(- 1)^{N + 1}}{2 \sqrt{N}}  \sum_{k = 0}^{\infty} \frac{(-
  1)^k}{k!} \left. \frac{d^k \Phi}{dz^k} \right|_{z = 2 (\sqrt{\frac{t}{2
  \pi}} - N) - 1} \left( \frac{1}{2 \pi} \right)^{k / 2} t^{- k / 2}
\end{equation}
Where $\Phi (z)$ is defined as:
\begin{equation}
  \Phi (z) = \frac{\cos (\pi (z^2 / 2 + 3 / 8))}{\cos (\pi z)}
\end{equation}

\section*{Derivation}

Starting with Riemann's integral representation:
\begin{equation}
  \pi^{- s / 2} \Gamma (s / 2) \zeta (s) = \int_0^{\infty} x^{s / 2 - 1} e^{-
  \pi x} dx + \int_{0 \swarrow 1} \frac{x^{- s} e^{\pi ix^2}}{e^{\pi ix} -
  e^{- \pi ix}} dx
\end{equation}
The saddle point occurs where:
\begin{equation}
  \frac{d}{dx}  (- s \log x + \pi ix^2) = 0
\end{equation}
giving $x = \sqrt{\frac{t}{2 \pi}}$. The integral from $N$ to $\infty$
transforms under $u = x - N$ to:
\begin{equation}
  \int_N^{\infty} e^{- 2 \pi i (x^2 - tx)} dx = e^{2 \pi i (N^2 - tN)} 
  \int_0^{\infty} e^{- 2 \pi i (u^2 + 2 Nu)} du
\end{equation}
By Watson's lemma:
\begin{equation}
  \int_0^{\infty} e^{- 2 \pi i (u^2 + 2 Nu)} du = \frac{e^{- \pi i / 4}}{2
  \sqrt{\pi}}  \sum_{k = 0}^{\infty} \frac{\Gamma (k + 1 / 2)}{k! (4 \pi
  iN)^k}
\end{equation}
The phase factor combines as:
\begin{equation}
  e^{2 \pi i (N^2 - tN)}  \frac{e^{- \pi i / 4}}{2 \sqrt{\pi}} = e^{\pi i (2
  N^2 - 2 tN - 1 / 4)}
\end{equation}
This leads to the function $\Phi (z)$ through the substitution $z = 2
(\sqrt{\frac{t}{2 \pi}} - N) - 1$, and the remainder term $R (t)$ emerges in
its final form as given above. The functional equation of zeta provides the
second main sum term:
\begin{equation}
  \chi (t)  \sum_{n = 1}^N \frac{1}{n^{1 / 2 - it}}
\end{equation}
Combining all terms gives the complete Riemann-Siegel formula.

\end{document}
