\documentclass{article}
\usepackage[english]{babel}
\usepackage{amsmath,amssymb,amsthm}
\usepackage{geometry}
\geometry{margin=1in}

\newtheorem{definition}{Definition}
\newtheorem{theorem}{Theorem}
\newtheorem{corollary}{Corollary}

\begin{document}

\section*{Oscillatory Processes with Monotonic Phase Functions}

\begin{definition}[Oscillatory Process]
Let $\{X_t\}_{t\in\mathbb{R}}$ be a complex second-order process. $\{X_t\}$ is called oscillatory if
\[
X_t = \int_{-\infty}^\infty \phi_t(\omega)\,dZ(\omega),
\]
where $Z(\omega)$ has orthogonal increments and $E|dZ(\omega)|^2 = d\mu(\omega)$, and $\phi_t(\omega) = A_t(\omega) e^{i\omega t}$.
\end{definition}

\begin{theorem}
Let $\theta:\mathbb{R}\to\mathbb{R}$ be smooth and strictly monotonically increasing. Define
\[
\phi_t(\omega) = e^{i\omega\theta(t)} .
\]
Set
\[
A_t(\omega) = e^{i\omega(\theta(t)-t)} .
\]
Then the time-varying impulse response $h_t(u)$ defined by
\[
A_t(\omega) = \int_{-\infty}^\infty e^{i\omega u} h_t(u)\,du
\]
is
\[
h_t(u) = \delta(u - [\theta(t) - t]) .
\]
\end{theorem}

\begin{proof}
The inverse Fourier transform yields
\begin{align*}
h_t(u) &= \frac{1}{2\pi}\int_{-\infty}^\infty e^{-i\omega u}A_t(\omega)\,d\omega \\
       &= \frac{1}{2\pi}\int_{-\infty}^\infty e^{-i\omega u} e^{i\omega(\theta(t)-t)} d\omega \\
       &= \frac{1}{2\pi}\int_{-\infty}^\infty e^{i\omega(\theta(t)-t-u)}d\omega \\
       &= \delta(\theta(t)-t-u) \\
       &= \delta(u - [\theta(t)-t]) .
\end{align*}
\end{proof}

\begin{corollary}
Let $S_t = \int_{-\infty}^{\infty} e^{i\omega t} dZ(\omega)$. Then
\[
X_t = \int_{-\infty}^\infty S_{t-u}\,h_t(u)\,du = S_{2t - \theta(t)}
\]
and
\[
X_t = \int_{-\infty}^\infty e^{i\omega\theta(t)}\,dZ(\omega) .
\]
\end{corollary}

\begin{proof}
By the sifting property of the Dirac delta,
\begin{align*}
X_t &= \int_{-\infty}^\infty S_{t-u} \delta(u - [\theta(t)-t])\,du \\
    &= S_{t - [\theta(t)-t]} \\
    &= S_{2t - \theta(t)} .
\end{align*}
By direct substitution, the oscillatory representation holds by definition.
\end{proof}

\end{document}
