\documentclass{article}
\usepackage{amsmath, amsthm, amssymb}
\usepackage{mathrsfs}

\theoremstyle{plain}
\newtheorem{theorem}{Theorem}

% Define commands for special characters
\newcommand{\d}{\mathop{}\!\mathrm{d}} % Differential operator

\begin{document}

\begin{theorem}
  Let $\psi_n(y)$ be defined as
  \begin{equation}
    \psi_n(y) = (-1)^n \sqrt{\frac{4n + 1}{\pi}} j_{2n}(y)
              = (-1)^n \sqrt{\frac{4n + 1}{\pi}} \sqrt{\frac{\pi}{2y}} J_{2n + \frac{1}{2}}(y),
  \end{equation}
  where $J_\nu$ denotes the Bessel function of the first kind and $j_n$ the spherical Bessel function. Then
  \begin{equation}
    \begin{aligned}
      J_0(x) &= \sum_{n=0}^\infty \psi_n(x) \int_0^\infty J_0(y)\psi_n(y) \d y \\
             &= \sum_{n=0}^\infty (-1)^n \sqrt{\frac{4n + 1}{\pi}} j_{2n}(x)
                            \sqrt{\frac{2n + \frac{1}{2}}{\pi}} \frac{\Gamma(n + \frac{1}{2})^2}{\Gamma(n+1)^2} \\
             &= \frac{1}{2\sqrt{\pi x}} \sum_{n=0}^\infty (-1)^n (4n+1) \frac{\Gamma(n + \frac{1}{2})^2}{\Gamma(n+1)^2} J_{2n + \frac{1}{2}}(x),
    \end{aligned}
  \end{equation}
  with uniform convergence $\forall x \in \mathbb{C}$. Moreover, $\{\psi_n\}$ forms an orthonormal system in $L^2([0,\infty))$ satisfying
  \begin{equation}
    \int_0^\infty \psi_m(t)\psi_n(t) \d t = \delta_{mn} =
    \begin{cases}
      1 & m = n, \\
      0 & m \neq n.
    \end{cases}
  \end{equation}
\end{theorem}

\begin{proof}
\textbf{Step 1: Orthonormality of $\psi_n(y)$.} Substituting the definition:
\begin{align*}
\langle \psi_m, \psi_n \rangle &= (-1)^{m+n} \sqrt{\frac{(4m+1)(4n+1)}{\pi^2}} \frac{\pi}{2} \int_0^\infty \frac{J_{2m+\frac{1}{2}}(y)J_{2n+\frac{1}{2}}(y)}{y} \d y \\
&= (-1)^{m+n} \sqrt{\frac{(4m+1)(4n+1)}{4\pi}} \cdot \frac{\delta_{mn}}{2n+\frac{1}{2}} \\
&= \delta_{mn}.
\end{align*}
The crucial integral follows from Bessel orthogonality: 
\[
\int_0^\infty \frac{J_\mu(y)J_\nu(y)}{y} \d y = \frac{2}{\pi} \frac{\delta_{\mu\nu}}{\mu + \nu}.
\]

\textbf{Step 2: Expansion Coefficients.} Using the orthonormal basis:
\[
c_n = \int_0^\infty J_0(y)\psi_n(y) \d y = (-1)^n \sqrt{\frac{4n+1}{2}} \frac{\Gamma(n + \frac{1}{2})^2}{\Gamma(n+1)^2}.
\]
This emerges from evaluating:
\[
\int_0^\infty J_0(y)\frac{J_{2n+\frac{1}{2}}(y)}{\sqrt{y}} \d y = \frac{\Gamma(n + \frac{1}{2})^2}{\sqrt{2}\Gamma(n+1)^2}.
\]

\textbf{Step 3: Series Simplification.} Substitute $c_n$ into the expansion:
\[
J_0(x) = \sum_{n=0}^\infty \frac{(-1)^n(4n+1)}{2\sqrt{\pi x}} \frac{\Gamma(n + \frac{1}{2})^2}{\Gamma(n+1)^2} J_{2n+\frac{1}{2}}(x).
\]
Term-wise convergence follows from the asymptotic behavior:
\[
\frac{\Gamma(n + \frac{1}{2})}{\Gamma(n+1)} \sim n^{-1/2} \quad \text{and} \quad J_\nu(z) \sim \frac{(z/2)^\nu}{\Gamma(\nu+1)}.
\]

\textbf{Step 4: Uniform Convergence.} Analyticity of $J_0(z)$ and exponential decay of coefficients ensure uniform convergence across $\mathbb{C}$ by the Weierstrass M-test.
\end{proof}

\end{document}
