\documentclass{article}
\usepackage{amsmath, amssymb, amsthm}

\newtheorem{theorem}{Theorem}
\newtheorem{lemma}{Lemma}

\title{Eigenfunctions in RKHS with Specific Orthonormal Basis}
\author{}
\date{}

\begin{document}

\maketitle

\begin{theorem}
Let $K(t-s)$ be a stationary positive definite kernel with spectral density $S(\omega)$, and let $h(t) = \mathcal{F}^{-1}\{\sqrt{S(\omega)}\}(t)$. Let $\{\phi_i\}$ be an orthonormal basis for $L^2(\mathbb{R})$ such that:  
\[
K(t) = \sum_{i=0}^\infty \langle K, \phi_i \rangle \phi_i(t),
\]  
with uniform convergence on $\mathbb{R}$. Then:  
\begin{enumerate}
    \item $\psi_i(t) = (h * \phi_i)(t)$ form an orthonormal basis for the RKHS $\mathcal{H}_K$.
    \item $\psi_i$ are eigenfunctions of the integral operator $T_K$ with eigenvalues $\lambda_i = \langle K, \phi_i \rangle$.
\end{enumerate}
\end{theorem}

\begin{proof}
\textbf{1. Orthonormality and completeness of $\{\psi_i\}$ in $\mathcal{H}_K$:}  
The RKHS $\mathcal{H}_K$ is isometrically isomorphic to $L^2(\mathbb{R})$ under $g \mapsto h * g$, with inner product:  
\[
\langle f, g \rangle_{\mathcal{H}_K} = \langle h^{-1} * f, h^{-1} * g \rangle_{L^2}.
\]  
For $\psi_i = h * \phi_i$, we have:  
\[
\langle \psi_i, \psi_j \rangle_{\mathcal{H}_K} = \langle \phi_i, \phi_j \rangle_{L^2} = \delta_{ij}.
\]  
Completeness follows as any $f \in \mathcal{H}_K$ can be written as $f = h * g$ for $g \in L^2(\mathbb{R})$:
\[
g = \sum_{i=0}^\infty \langle g, \phi_i \rangle \phi_i \implies f = \sum_{i=0}^\infty \langle g, \phi_i \rangle (h * \phi_i) = \sum_{i=0}^\infty \langle f, \psi_i \rangle_{\mathcal{H}_K} \psi_i.
\]  

\textbf{2. Eigenfunction Property of $\psi_i$:}  
The integral operator $T_K$ is defined as:  
\[
(T_K f)(t) = \int_{-\infty}^\infty K(t-s)f(s)ds = (K * f)(t).
\]  
Using the kernel's expansion $K = \sum_{i=0}^\infty \lambda_i \phi_i$ where $\lambda_i = \langle K, \phi_i \rangle$, we have:  
\[
T_K \psi_j = K * (h * \phi_j) = (K * h) * \phi_j.
\]  
The spectral factorization gives $K = h * h^*$. Crucially, the uniform convergence hypothesis ensures that convolution with $K$ commutes with the basis decomposition:
\[
K * \phi_j = \sum_{i=0}^\infty \lambda_i \langle \phi_j, \phi_i \rangle \phi_i = \lambda_j \phi_j.
\]  
Therefore:
\[
T_K \psi_j = h * (K * \phi_j) = h * (\lambda_j \phi_j) = \lambda_j (h * \phi_j) = \lambda_j \psi_j.
\]  
This confirms $\psi_j$ are eigenfunctions of $T_K$ with eigenvalues $\lambda_j$.  
\end{proof}

\end{document}
