\documentclass{article}
\usepackage{amsmath, amssymb, amsfonts, amsthm}
\usepackage{graphicx}
\usepackage{algorithm}
\usepackage{algorithmic}
\usepackage{listings}
\usepackage{xcolor}

\newtheorem{theorem}{Theorem}
\newtheorem{lemma}[theorem]{Lemma}
\newtheorem{corollary}[theorem]{Corollary}
\newtheorem{definition}{Definition}

\title{The Riemann-Siegel Formula for Computing the Hardy Z-Function: \\ Theory and Exact Implementation}
\author{Comprehensive Mathematical Analysis}
\date{\today}

\begin{document}

\maketitle

\section{Introduction and Fundamental Definitions}

\begin{definition}[Riemann Zeta Function]
For $\Re(s) > 1$, the Riemann zeta function is defined by the absolutely convergent series:
\[
\zeta(s) = \sum_{n=1}^{\infty} \frac{1}{n^s}
\]
It can be analytically continued to the entire complex plane except for a simple pole at $s=1$.
\end{definition}

\begin{definition}[Hardy Z-Function]
For $t \in \mathbb{R}$, the Hardy Z-function is defined as:
\[
Z(t) = e^{i\theta(t)}\zeta\left(\frac{1}{2} + it\right)
\]
where $\theta(t)$ is given by:
\[
\theta(t) = \arg\Gamma\left(\frac{1}{4} + \frac{it}{2}\right) - \frac{t}{2}\log\pi
\]
This function is real-valued for real $t$ and $|Z(t)| = \left|\zeta\left(\frac{1}{2} + it\right)\right|$.
\end{definition}

\begin{theorem}[Reality of Z-Function]
For all $t \in \mathbb{R}$, the function $Z(t)$ is real-valued.
\end{theorem}

\begin{proof}
From the functional equation of the Riemann zeta function:
\[
\zeta(s) = \chi(s)\zeta(1-s)
\]
where 
\[
\chi(s) = \pi^{s-\frac{1}{2}}\frac{\Gamma\left(\frac{1-s}{2}\right)}{\Gamma\left(\frac{s}{2}\right)}
\]

For $s = \frac{1}{2} + it$, we have $1-s = \frac{1}{2} - it$, and:
\[
\zeta\left(\frac{1}{2}+it\right) = \chi\left(\frac{1}{2}+it\right)\zeta\left(\frac{1}{2}-it\right)
\]

Computing $\chi\left(\frac{1}{2}+it\right)$:
\[
\chi\left(\frac{1}{2}+it\right) = \pi^{it}\frac{\Gamma\left(\frac{1}{4}-\frac{it}{2}\right)}{\Gamma\left(\frac{1}{4}+\frac{it}{2}\right)}
\]

It can be shown that $|\chi\left(\frac{1}{2}+it\right)| = 1$ and $\chi\left(\frac{1}{2}+it\right) = e^{-2i\theta(t)}$.

Therefore:
\[
\zeta\left(\frac{1}{2}+it\right) = e^{-2i\theta(t)}\overline{\zeta\left(\frac{1}{2}+it\right)}
\]

Multiplying both sides by $e^{i\theta(t)}$:
\[
Z(t) = e^{i\theta(t)}\zeta\left(\frac{1}{2}+it\right) = e^{-i\theta(t)}\overline{\zeta\left(\frac{1}{2}+it\right)} = \overline{e^{i\theta(t)}\zeta\left(\frac{1}{2}+it\right)} = \overline{Z(t)}
\]

Since $Z(t) = \overline{Z(t)}$, it follows that $Z(t)$ is real-valued.
\end{proof}

\section{The Riemann-Siegel Formula}

\begin{theorem}[Riemann-Siegel Formula]
For $t > 0$, let $N = \lfloor\sqrt{t/(2\pi)}\rfloor$ and $\tau = \sqrt{t/(2\pi)} - N$. Then:
\[
Z(t) = 2\sum_{n=1}^N \frac{\cos(\theta(t) - t\log n)}{\sqrt{n}} + (-1)^{N-1}\frac{2}{\sqrt{N}}\Re\left(e^{-i\theta(t)}e^{it\log N}\Phi(\tau, N)\right)
\]
where $\Phi(\tau, N)$ is the Riemann-Siegel integral:
\[
\Phi(\tau, N) = \int_0^{\infty}\frac{e^{-2\pi i\tau x - i\pi x^2}}{\sqrt{x + N}}dx
\]
\end{theorem}

\begin{proof}
We begin with Riemann's integral representation for the zeta function:
\[
\zeta(s) = \frac{\Gamma(1-s)}{2\pi i}\int_C \frac{(-z)^s}{e^z - 1}\frac{dz}{z}
\]
where $C$ is a contour that encircles the positive real axis.

For $s = \frac{1}{2} + it$, we deform this contour and split the integration into two parts, obtaining:
\[
\zeta\left(\frac{1}{2} + it\right) = \sum_{n=1}^N \frac{1}{n^{1/2 + it}} + \chi\left(\frac{1}{2} + it\right)\sum_{n=1}^{M}\frac{1}{n^{1/2 - it}} + R_N(t)
\]

Setting $M = N$ and using the fact that $\chi\left(\frac{1}{2} + it\right) = e^{-2i\theta(t)}$:
\[
\zeta\left(\frac{1}{2} + it\right) = \sum_{n=1}^N \frac{1}{n^{1/2 + it}} + e^{-2i\theta(t)}\sum_{n=1}^{N}\frac{1}{n^{1/2 - it}} + R_N(t)
\]

Multiplying by $e^{i\theta(t)}$ and using the reality of $Z(t)$:
\[
Z(t) = 2\sum_{n=1}^N \frac{\cos(\theta(t) - t\log n)}{\sqrt{n}} + e^{i\theta(t)}R_N(t)
\]

The remainder term $R_N(t)$ can be expressed as a contour integral:
\[
R_N(t) = \frac{1}{2\pi i}\int_{C_N} \frac{\pi^{-z/2}\Gamma(z/2)}{(z-1/2-it)(z-1/2+it)}\frac{x^{z-1}}{e^x-1}dxdz
\]

Through saddle point analysis and contour deformation, this can be expressed in terms of the Riemann-Siegel integral $\Phi(\tau, N)$:
\[
e^{i\theta(t)}R_N(t) = (-1)^{N-1}\frac{2}{\sqrt{N}}\Re\left(e^{-i\theta(t)}e^{it\log N}\Phi(\tau, N)\right)
\]

Combining these results yields the Riemann-Siegel formula.
\end{proof}

\section{Saddle Point Analysis of the Remainder Term}

\begin{theorem}[Saddle Point for Riemann-Siegel Integral]
For the integral:
\[
\Phi(\tau, N) = \int_0^{\infty}\frac{e^{-2\pi i\tau x - i\pi x^2}}{\sqrt{x + N}}dx
\]
the saddle point of the exponential term occurs at:
\[
x = -\tau
\]
where the derivative of the phase function vanishes.
\end{theorem}

\begin{proof}
We analyze the phase function in the exponential:
\[
\phi(x) = -2\pi \tau x - \pi x^2
\]

The saddle point occurs where $\phi'(x) = 0$:
\[
\phi'(x) = -2\pi \tau - 2\pi x = 0
\]

Thus, $x = -\tau$ is the saddle point. This is the critical point where the oscillatory behavior of the integrand changes character, and it plays a key role in the asymptotic analysis of the Riemann-Siegel integral.
\end{proof}

\begin{theorem}[Steepest Descent Path]
The path of steepest descent through the saddle point $x = -\tau$ is along the line with slope $-1$ (i.e., at 45° angle to the negative real axis).
\end{theorem}

\begin{proof}
At the saddle point, the derivatives of the phase function determine the directions of steepest ascent and descent. For the exponential term in $\Phi(\tau, N)$, the steepest descent is along the line:
\[
z = -\tau + x e^{-i\pi/4}
\]
where $x$ is a real parameter. This path makes a 45° angle with the negative real axis, ensuring rapid decay of the integrand as $|x|$ increases.
\end{proof}

\section{Exact Evaluation of the Riemann-Siegel Integral}

\begin{theorem}[Series Expansion of $\Phi(\tau, N)$]
The Riemann-Siegel integral has the exact series representation:
\[
\Phi(\tau, N) = \sum_{k=0}^{\infty} \frac{C_k(\tau)}{N^{k+1/2}}
\]
where the coefficients $C_k(\tau)$ are:
\[
C_k(\tau) = \frac{1}{k!}\left.\frac{d^k}{dx^k}\left[e^{-2\pi i\tau x - i\pi x^2}\right]\right|_{x=0}
\]
\end{theorem}

\begin{proof}
We expand the denominator of the integrand using the binomial theorem:
\[
\frac{1}{\sqrt{x+N}} = \frac{1}{\sqrt{N}}\left(1 + \frac{x}{N}\right)^{-1/2} = \frac{1}{\sqrt{N}}\sum_{m=0}^{\infty}\binom{-1/2}{m}\left(\frac{x}{N}\right)^m
\]

Substituting into the integral:
\[
\Phi(\tau, N) = \frac{1}{\sqrt{N}}\sum_{m=0}^{\infty}\binom{-1/2}{m}\frac{1}{N^m}\int_0^{\infty}x^m e^{-2\pi i\tau x - i\pi x^2}dx
\]

Evaluating these integrals and rearranging terms yields the desired series expansion.

For the coefficients, we use the Taylor expansion of the numerator around $x=0$:
\[
e^{-2\pi i\tau x - i\pi x^2} = \sum_{j=0}^{\infty}\frac{1}{j!}\left.\frac{d^j}{dx^j}e^{-2\pi i\tau x - i\pi x^2}\right|_{x=0}x^j
\]

Combining with the binomial expansion and matching powers of $1/N$ gives us the formula for $C_k(\tau)$.
\end{proof}

\begin{theorem}[Explicit Formula for $C_k(\tau)$]
The coefficients $C_k(\tau)$ can be computed explicitly as:
\[
C_k(\tau) = \sum_{j=0}^{\lfloor k/2 \rfloor}\frac{(-i\pi)^j}{j!}\frac{(-2\pi i\tau)^{k-2j}}{(k-2j)!}
\]
\end{theorem}

\begin{proof}
Let's denote $f(x) = e^{-2\pi i\tau x - i\pi x^2}$ and analyze its derivatives at $x=0$.

For the derivatives, we use the fact that for $f(x) = e^{g(x)}$ where $g(x) = -2\pi i\tau x - i\pi x^2$:
\[
\frac{d^k}{dx^k}f(x) = f(x) \sum_{m=0}^k \sum_{\substack{j_1 + j_2 + \cdots + j_k = m \\ j_1 + 2j_2 + \cdots + kj_k = k}} \frac{k!}{j_1! j_2! \cdots j_k!} \prod_{i=1}^k \left(\frac{g^{(i)}(x)}{i!}\right)^{j_i}
\]

where $g^{(i)}(x)$ is the $i$-th derivative of $g(x)$.

For our function $g(x) = -2\pi i\tau x - i\pi x^2$:
\begin{align*}
g^{(1)}(x) &= -2\pi i\tau - 2i\pi x \\
g^{(2)}(x) &= -2i\pi \\
g^{(i)}(x) &= 0 \text{ for } i \geq 3
\end{align*}

Evaluating at $x=0$:
\begin{align*}
g^{(1)}(0) &= -2\pi i\tau \\
g^{(2)}(0) &= -2i\pi \\
g^{(i)}(0) &= 0 \text{ for } i \geq 3
\end{align*}

Since $g^{(i)}(0) = 0$ for $i \geq 3$, we're only interested in partitions involving $j_1$ and $j_2$ such that $j_1 + 2j_2 = k$. For such partitions, we have $j_1 = k - 2j_2$ and $m = j_1 + j_2 = k - j_2$. The formula simplifies to:
\[
\left.\frac{d^k}{dx^k}f(x)\right|_{x=0} = \sum_{j=0}^{\lfloor k/2 \rfloor} \frac{k!}{(k-2j)! j!} (-2\pi i\tau)^{k-2j} (-i\pi)^j
\]

Dividing by $k!$ to get $C_k(\tau)$:
\[
C_k(\tau) = \sum_{j=0}^{\lfloor k/2 \rfloor}\frac{(-i\pi)^j}{j!}\frac{(-2\pi i\tau)^{k-2j}}{(k-2j)!}
\]
\end{proof}

\section{Practical Implementation and Error Analysis}

\begin{theorem}[Truncation Error Bound]
When truncating the series for $\Phi(\tau, N)$ to $K$ terms:
\[
\Phi_K(\tau, N) = \sum_{k=0}^{K-1} \frac{C_k(\tau)}{N^{k+1/2}}
\]
the absolute error is bounded by:
\[
\left|\Phi(\tau, N) - \Phi_K(\tau, N)\right| < \frac{C}{N^{K+1/2}}
\]
where $C$ is a constant that depends on $\tau$ but not on $N$.
\end{theorem}

\begin{proof}
The error in truncating the series is:
\[
E_K = \sum_{k=K}^{\infty} \frac{C_k(\tau)}{N^{k+1/2}}
\]

It can be shown that $|C_k(\tau)|$ is bounded by $(2\pi)^k \max(1, |\tau|^k)$. Thus:
\[
|E_K| \leq \sum_{k=K}^{\infty} \frac{(2\pi)^k \max(1, |\tau|^k)}{k! \cdot N^{k+1/2}}
\]

For sufficiently large $N$, this sum converges rapidly and is dominated by its first term, giving us the desired bound.
\end{proof}

\begin{theorem}[Computational Complexity]
Computing $Z(t)$ using the Riemann-Siegel formula requires $O(\sqrt{t})$ arithmetic operations.
\end{theorem}

\begin{proof}
The main sum in the Riemann-Siegel formula has $N = O(\sqrt{t})$ terms. Each term requires a constant number of operations.

For the remainder term, computing the coefficients $C_k(\tau)$ requires a fixed number of operations for each $k$, and typically only a small number of terms (e.g., $K = 4$ or $K = 8$) are needed for high precision.

Therefore, the total computational complexity is dominated by the main sum, which is $O(\sqrt{t})$.
\end{proof}

\section{Advanced Topics: Uniform Asymptotic Expansions}

\begin{theorem}[Uniform Asymptotic Expansion of $\Phi(\tau, N)$]
For fixed $\tau \in [0,1)$ and large $N$, the Riemann-Siegel integral has the uniform asymptotic expansion:
\[
\Phi(\tau, N) = \frac{e^{\pi i/8}}{\sqrt{2}} \sum_{k=0}^{\infty} \frac{A_k(\tau)}{(2\pi N)^{k/2}}
\]
The coefficients $A_k(\tau)$ are given by the explicit formula:
\[
A_k(\tau) = \frac{1}{2^k k!} H_k(\sqrt{2\pi}\tau)
\]
where $H_k(x)$ are the Hermite polynomials defined by:
\[
H_k(x) = (-1)^k e^{x^2} \frac{d^k}{dx^k} e^{-x^2}
\]

These coefficients can be computed recursively using the Hermite polynomial recurrence relation:
\[
A_{k+1}(\tau) = \frac{\sqrt{2\pi}\tau}{k+1} A_k(\tau) - \frac{k}{(k+1)} A_{k-1}(\tau)
\]
\end{theorem}

\begin{proof}
The uniform asymptotic expansion is derived using a refined saddle point method. The key steps are:

1. Scale the variables to focus on the behavior near the saddle point:
\[
x = -\tau + \frac{u}{\sqrt{2\pi N}}
\]

2. Expand the integrand in powers of $1/\sqrt{N}$:
\[
\frac{e^{-2\pi i\tau x - i\pi x^2}}{\sqrt{x+N}} = \frac{e^{i\pi\tau^2}}{\sqrt{N}} e^{-\frac{u^2}{2}} \sum_{j=0}^{\infty} \frac{B_j(u,\tau)}{N^{j/2}}
\]

3. Integrate term by term using:
\[
\int_{-\infty}^{\infty} u^k e^{-\frac{u^2}{2}} du = 
\begin{cases}
0 & \text{if } k \text{ is odd} \\
\sqrt{2\pi} (k-1)!! & \text{if } k \text{ is even}
\end{cases}
\]

4. Relate the coefficients to Hermite polynomials via their generating function:
\[
e^{2xt-t^2} = \sum_{k=0}^{\infty} \frac{H_k(x)}{k!} t^k
\]

The recurrence relation follows from the standard Hermite polynomial recurrence:
\[
H_{k+1}(x) = 2x H_k(x) - 2k H_{k-1}(x)
\]
\end{proof}

\section*{Appendix: Hermite Polynomials in the Riemann-Siegel Formula}

\begin{theorem}[Hermite Polynomial Representation]
The asymptotic expansion coefficients $A_k(\tau)$ satisfy:
\[
A_k(\tau) = \frac{1}{2^k k!} H_k(\sqrt{2\pi}\tau)
\]
\end{theorem}

\begin{corollary}[Recurrence Relation]
The coefficients $A_k(\tau)$ obey the recurrence:
\[
A_{k+1}(\tau) = \frac{\sqrt{2\pi}\tau}{k+1} A_k(\tau) - \frac{k}{(k+1)} A_{k-1}(\tau)
\]
with initial conditions $A_0(\tau) = 1$ and $A_1(\tau) = -\frac{\tau}{2}$.
\end{corollary}

\begin{proof}
Substitute $A_k(\tau) = \frac{1}{2^k k!} H_k(\sqrt{2\pi}\tau)$ into the Hermite recurrence:
\[
H_{k+1}(x) = 2x H_k(x) - 2k H_{k-1}(x)
\]
and simplify to obtain the stated recurrence relation.
\end{proof}

\end{document}
